src/Term_Defs.v
@@ -35,7 +35,7 @@ Set Nested Proofs Allowed.
 (** [Plc] represents a place. *)
 
 Notation Plc := nat (only parsing).
-Notation Loc := nat (only parsing).
+(*Notation Loc := nat (only parsing). *)
 Notation ASP_ID := nat (only parsing).
 Notation N_ID := nat (only parsing).
 Notation Arg := nat (only parsing).
@@ -59,7 +59,9 @@ Inductive Term: Set :=
 (*| bseq: Split -> Term -> Term -> Term
 | bpar: Split -> Term -> Term -> Term*) .
 
+(*
 Definition LocRange: Set := list Loc.
+
 
 Definition getTwoLocs (ls:list Loc) (b:bool): option (Loc*Loc) :=
   match b with
@@ -70,6 +72,7 @@ Definition getTwoLocs (ls:list Loc) (b:bool): option (Loc*Loc) :=
     end
   | false => ret (0,0)
   end.
+*)
 
 (** The structure of evidence. *)
 
@@ -124,8 +127,8 @@ Inductive Ev: Set :=
 | umeas: nat -> Plc -> ASP_ID -> list Arg -> Ev
 | sign: nat -> Plc -> Ev
 (*| hash: nat -> Plc -> Ev *)
-| req: nat -> Loc -> Plc -> Plc -> Term -> Ev
-| rpy: nat -> Loc -> Plc -> Plc -> Ev 
+| req: nat -> (*Loc ->*) Plc -> Plc -> Term -> Ev
+| rpy: nat -> (*Loc -> *) Plc -> Plc -> Ev 
 | split: nat -> Plc -> Ev
 (*| splitp: nat -> (*Loc ->*) Loc -> Plc -> Ev *)
 | join:  nat -> Plc -> Ev
@@ -147,8 +150,8 @@ Definition ev x : nat :=
   | umeas i _ _ _  => i
   | sign i _ => i
   (*| hash i _ => i *)
-  | req i _ _ _ _ => i
-  | rpy i _ _ _ => i 
+  | req i _ _ _ => i
+  | rpy i _ _ => i 
   | split i _ => i
   (* | splitp i _ _ => i *)
   | join i _ => i
@@ -156,14 +159,14 @@ Definition ev x : nat :=
   end.
 
 (** The natural number indicating the place where an event occured. *)
-Definition pl x : Loc :=
+Definition pl x : Plc :=
   match x with
   | copy _ p => p
   | umeas _ p _ _  => p
   | sign _ p => p
   (*| hash _ p => p *)
-  | req _ _ p _ _ => p
-  | rpy _ _ p _ => p
+  | req _ p _ _ => p
+  | rpy _ p _ => p
   | split _ p => p
   (*| splitp _ _ p => p *)
   | join _ p => p
@@ -199,30 +202,31 @@ Definition asp_event i x p :=
 Definition Range: Set := nat * nat.
 
 Inductive AnnoTerm: Set :=
-| aasp: Range -> LocRange -> ASP -> AnnoTerm
-| aatt: Range -> LocRange -> (Loc*Loc) -> Plc -> AnnoTerm -> AnnoTerm
-| alseq: Range -> LocRange -> AnnoTerm -> AnnoTerm -> AnnoTerm
+| aasp: Range -> (*LocRange ->*) ASP -> AnnoTerm
+| aatt: Range -> (*LocRange -> (Loc*Loc) ->*) Plc -> AnnoTerm -> AnnoTerm
+| alseq: Range -> (*LocRange ->*) AnnoTerm -> AnnoTerm -> AnnoTerm
 (*| abseq: Range -> LocRange -> Split -> AnnoTerm -> AnnoTerm -> AnnoTerm
 | abpar: Range -> LocRange -> (*(Loc*Loc) ->*) (Loc*Loc) -> Split -> AnnoTerm -> AnnoTerm -> AnnoTerm*) .
 
 Fixpoint esize t :=
   match t with
-  | aasp _ _ _ => 1
-  | aatt _ _ _ _ t1 => 2 + (*remote_esize t1*) esize t1
-  | alseq _ _ t1 t2 => esize t1 + esize t2
+  | aasp _ _ => 1
+  | aatt _ _ t1 => 2 + (*remote_esize t1*) esize t1
+  | alseq _ t1 t2 => esize t1 + esize t2
   (*| abseq _ _ _ t1 t2 => 2 + esize t1 + esize t2
   | abpar _ _ _ _ t1 t2 => 2 + esize t1 + esize t2 *)
   end.
 
 Definition range x :=
   match x with
-  | aasp r _ _ => r
-  | aatt r _ _ _ _ => r
-  | alseq r _ _ _ => r
+  | aasp r _ => r
+  | aatt r _ _ => r
+  | alseq r _ _ => r
   (*| abseq r _ _ _ _ => r
   | abpar r _ _ _ _ _ => r *)
   end.
 
+(*
 Definition lrange x :=
   match x with
   | aasp _ lr _ => lr
@@ -285,26 +289,25 @@ Proof.
     assert (Nat.even (nss t2) = true) by eauto.
     eapply both_args_even; eauto. *)
 Defined.
+*)
 
 (*
 (** This function annotates a term.  It feeds a natural number
     throughout the computation so as to ensure each event has a unique
     natural number. *) *)
 
-Fixpoint anno (t: Term) (i:nat) (ls:LocRange) (b:bool) : option (nat * (* (LocRange **) AnnoTerm)(* ) *) :=
+Fixpoint anno (t: Term) (i:nat) : (nat * AnnoTerm) :=
   match t with
-  | asp x => ret (S i, (aasp (i, S i) [] x))
+  | asp x => (S i, (aasp (i, S i) x))
 
   | att p x =>
-    '(req_loc,rpy_loc) <- getTwoLocs ls b ;;
-    '(j,a) <- anno x (S i) [] false  ;;
-    (* TODO: does ls matter here?  Should it be []? *)
-    ret (S j, aatt (i, S j) (firstn 2 ls) (req_loc,rpy_loc) p a)
+    let '(j,a) := anno x (S i)  in
+    (S j, aatt (i, S j) p a)
 
   | lseq x y =>
-    '(j,a) <- anno x i (firstn (nss x) ls) b  ;;
-    '(k,bt) <- anno y j (skipn (nss x) ls ) b  ;;
-    ret (k, alseq (i, k) ls (*(lrange a ++ lrange bt)*) a bt)
+    let '(j,a) := anno x i in
+    let '(k,bt) := anno y j in
+    (k, alseq (i, k) a bt)
 
         (*
   | bseq s x y =>
@@ -322,16 +325,18 @@ Fixpoint anno (t: Term) (i:nat) (ls:LocRange) (b:bool) : option (nat * (* (LocRa
 *)
   end.
 
+(*
 Definition anno' t i ls := fromSome (0, aasp (0,0) [] CPY) (anno t i ls true).
+*)
 
-Definition annotated x ls :=
-  snd (anno' x 0 ls).
+Definition annotated x :=
+  snd (anno x 0).
 
 Fixpoint unanno a :=
   match a with
-  | aasp _ _ a => asp a
-  | aatt _ _ _ p t => att p (unanno t)
-  | alseq _ _ a1 a2 => lseq (unanno a1) (unanno a2)
+  | aasp _ a => asp a
+  | aatt _ p t => att p (unanno t)
+  | alseq _ a1 a2 => lseq (unanno a1) (unanno a2)
                          
   (*| abseq _ _ spl a1 a2 => bseq spl (unanno a1) (unanno a2) 
   | abpar _ _ _ spl a1 a2 => bpar spl (unanno a1) (unanno a2) *)
@@ -354,22 +359,22 @@ Lemma unique_req_events (t:AnnoTerm) : forall p i i0 p1 p2 q q0 t0 t1,
  *)
 
 Inductive well_formed_r: AnnoTerm -> Prop :=
-| wf_asp_r: forall r x ls,
+| wf_asp_r: forall r x,
     snd r = S (fst r) ->
-    well_formed_r (aasp r ls x)
-| wf_att_r: forall r ls locs p x,
+    well_formed_r (aasp r x)
+| wf_att_r: forall r p x,
     well_formed_r x ->
     S (fst r) = fst (range x) ->
     snd r = S (snd (range x)) ->
     Nat.pred (snd r) > fst r ->
-    well_formed_r (aatt r ls locs p x)
+    well_formed_r (aatt r p x)
                   
-| wf_lseq_r: forall r ls x y,
+| wf_lseq_r: forall r x y,
     well_formed_r x -> well_formed_r y ->
     fst r = fst (range x) ->
     snd (range x) = fst (range y) ->
     snd r = snd (range y) -> 
-    well_formed_r (alseq r ls x y)
+    well_formed_r (alseq r x y)
    (*               
 | wf_bseq_r: forall r ls s x y,
     well_formed_r x -> well_formed_r y ->
@@ -387,6 +392,7 @@ Inductive well_formed_r: AnnoTerm -> Prop :=
     well_formed_r (abpar r ls (*xlocs*) ylocs s x y) *) .
 Hint Constructors well_formed_r : core.
 
+(*
 Inductive well_formed: AnnoTerm -> Prop :=
 | wf_asp: forall r x,
     snd r = S (fst r) ->
@@ -524,6 +530,7 @@ Inductive well_formed: AnnoTerm -> Prop :=
     (*length ls >= 4 + length (lrange x) + length (lrange y) ->*)
     well_formed (abpar r ls (*xlocs*) ylocs s x y) *) .
 Hint Constructors well_formed : core.
+*)
 
 Ltac afa :=
   match goal with   
