src/Helpers_VmSemantics.v
@@ -10,16 +10,16 @@ Require Import Coq.Program.Tactics Coq.Program.Equality.
 
 Set Nested Proofs Allowed.
 
-Lemma pl_immut : forall t e tr p o,
-    well_formed t ->
+Lemma pl_immut : forall t e tr p,
+    well_formed_r t ->
     st_pl
       (execSt
          (copland_compile t)
          {|
            st_ev := e;
            st_trace := tr;
-           st_pl := p;
-           st_store := o |}) = p.
+           st_pl := p(*;
+           st_store := o*) |}) = p.
 Proof.
   induction t; intros.
   -
@@ -27,7 +27,9 @@ Proof.
     destruct a;
       reflexivity.
   -
-    repeat (df; dohtac; df).
+    do_wf_pieces.
+    
+    repeat (df; try dohtac; df).   
     reflexivity.
   -
     do_wf_pieces.
@@ -284,25 +286,25 @@ Ltac do_pl_immut :=
       | [H: copland_compile ?t
             {| st_ev := _;
                         st_trace := _;
-                        st_pl := ?p;
-                        st_store := _ |} =
+                        st_pl := ?p (*;
+                        st_store := _ *) |} =
             (_,
              {| st_ev := _;
                          st_trace := _;
-                         st_pl := ?p';
-                                  st_store := _ |}),
-         H2: well_formed ?t |- _] =>
+                         st_pl := ?p' (*;
+                                  st_store := _*) |}),
+         H2: well_formed_r ?t |- _] =>
         assert_new_proof_by (p' = p) ltac:(tac H H2)  
       end.
 
 
 Lemma st_congr :
-  forall st tr e p o,
+  forall st tr e p,
     st_ev st = e ->
     st_trace st = tr ->
     st_pl st = p ->
-    st_store st = o ->
-    st =  {| st_ev := e; st_trace := tr; st_pl := p; st_store := o |}.
+    (*st_store st = o -> *)
+    st =  {| st_ev := e; st_trace := tr; st_pl := p (*; st_store := o*) |}.
 Proof.
   intros.
   subst; destruct st; auto.
@@ -322,23 +324,23 @@ Ltac allss :=
 Ltac anhl :=
   annogo;
   match goal with
-  | [H: well_formed ?a,
+  | [H: well_formed_r ?a,
      H2: copland_compile ?a _ = _,
      H3: copland_compile ?a _ = _,
-     IH: context[well_formed ?a (*copland_compile ?a _ = _ *) -> _] |- _] =>
+     IH: context[well_formed_r ?a (*copland_compile ?a _ = _ *) -> _] |- _] =>
     edestruct IH;
     [apply H | 
      apply H2 | apply H3 | idtac]; clear H2; clear H3;
     destruct_conjs; subst
   end.
 
-Lemma hihi : forall t e e' e'' x x' y y' p p' p'' o o' o'',
-    well_formed t ->
-    copland_compile t {| st_ev := e; st_trace := x; st_pl := p; st_store := o |} =
-    (Some tt, {| st_ev := e'; st_trace := x'; st_pl := p'; st_store := o' |}) ->
-    copland_compile t {| st_ev := e; st_trace := y; st_pl := p; st_store := o |} =
-    (Some tt, {| st_ev := e''; st_trace := y'; st_pl := p''; st_store := o'' |}) ->
-    (e' = e'' /\ p' = p'' /\ o' = o'').
+Lemma hihi : forall t e e' e'' x x' y y' p p' p'',
+    well_formed_r t ->
+    copland_compile t {| st_ev := e; st_trace := x; st_pl := p (*; st_store := o*) |} =
+    (Some tt, {| st_ev := e'; st_trace := x'; st_pl := p' (*; st_store := o'*) |}) ->
+    copland_compile t {| st_ev := e; st_trace := y; st_pl := p (*; st_store := o*) |} =
+    (Some tt, {| st_ev := e''; st_trace := y'; st_pl := p'' (*; st_store := o''*) |}) ->
+    (e' = e'' /\ p' = p'' (*/\ o' = o''*)).
 Proof.
   induction t; intros.
   - destruct a;
@@ -346,7 +348,7 @@ Proof.
   -
     (*
     do_wf_pieces. *)
-    repeat (df; dohtac; df).
+    repeat (df; try dohtac; df).
     tauto.
   -
     do_wf_pieces.
@@ -417,12 +419,12 @@ Ltac dohi'' :=
   annogo;
   let tac Hwf H H' := eapply hihi; [apply Hwf | apply H | apply H'] in
   match goal with
-  | [H : copland_compile ?t1 {| st_ev := ?e; st_trace := _; st_pl := ?p; st_store := ?o |} =
-         (?opt, {| st_ev := ?e'; st_trace := _; st_pl := ?p'; st_store := ?o' |}),
-         H' : copland_compile ?t1 {| st_ev := ?e; st_trace := _; st_pl := ?p; st_store := ?o |} =
-              (?opt, {| st_ev := ?e''; st_trace := _; st_pl := ?p''; st_store := ?o'' |}),
-                Hwf : well_formed ?t1  |- _] =>
-    assert_new_proof_by (e' = e'' /\ p' = p'' /\ o' = o'') ltac:(tac Hwf H H')
+  | [H : copland_compile ?t1 {| st_ev := ?e; st_trace := _; st_pl := ?p (*; st_store := ?o*) |} =
+         (?opt, {| st_ev := ?e'; st_trace := _; st_pl := ?p' (*; st_store := ?o'*) |}),
+         H' : copland_compile ?t1 {| st_ev := ?e; st_trace := _; st_pl := ?p (*; st_store := ?o*) |} =
+              (?opt, {| st_ev := ?e''; st_trace := _; st_pl := ?p'' (*; st_store := ?o''*) |}),
+                Hwf : well_formed_r ?t1  |- _] =>
+    assert_new_proof_by (e' = e'' /\ p' = p'' (*/\ o' = o''*)) ltac:(tac Hwf H H')
   end.
 
 Ltac dohi :=
@@ -431,6 +433,7 @@ Ltac dohi :=
 
 Require Import List_Facts.
 
+(*
 Lemma store_untouched : forall t st1 st1' store1 store1' x v,
     copland_compile t st1 = (Some tt, st1') ->
     store1 = st_store st1 ->
@@ -440,9 +443,10 @@ Lemma store_untouched : forall t st1 st1' store1 store1' x v,
     map_get store1' x = Some v.
 Proof.
 Admitted.
+*)
 
 Lemma always_some : forall t vm_st vm_st' op,
-    well_formed t ->
+    well_formed_r t ->
     copland_compile 
       t
       vm_st =
@@ -454,7 +458,7 @@ Proof.
     destruct a;
       try (df; tauto).
   -
-    repeat (df; dohtac; df).
+    repeat (df; try dohtac; df).
     tauto.
   -
     df. 
@@ -521,22 +525,23 @@ Defined.
 Ltac do_somett :=
   match goal with
   | [H: copland_compile ?t _ = (?o, _),
-        H2: well_formed ?t |- _] =>
+        H2: well_formed_r ?t |- _] =>
     assert_new_proof_by (o = Some tt) ltac:(eapply always_some; [apply H2 | apply H])
   end.
 
 
 Ltac do_asome := repeat do_somett; clear_triv.
 
-Lemma trace_irrel_store : forall t tr1 tr1' tr2 e e' p1' p1 o' o,
+(*
+Lemma trace_irrel_store : forall t tr1 tr1' tr2 e e' p1' p1,
     well_formed t ->
     copland_compile t
-           {| st_ev := e;  st_trace := tr1; st_pl := p1;  st_store := o  |} =
-    (Some tt, {| st_ev := e'; st_trace := tr1'; st_pl := p1'; st_store := o' |}) ->
+           {| st_ev := e;  st_trace := tr1; st_pl := p1 (*;  st_store := o*)  |} =
+    (Some tt, {| st_ev := e'; st_trace := tr1'; st_pl := p1' (*; st_store := o'*) |}) ->
     
     st_store
       (execSt (copland_compile t)
-           {| st_ev := e;  st_trace := tr2; st_pl := p1;  st_store := o  |}) = o'.
+           {| st_ev := e;  st_trace := tr2; st_pl := p1 (*; st_store := o*)  |}) = o'.
 Proof.
   intros.
   destruct (copland_compile t {| st_ev := e; st_trace := tr2; st_pl := p1; st_store := o |}) eqn:ff.
@@ -549,19 +554,20 @@ Proof.
   df.
   tauto.
 Defined.
+*)
 
-Lemma trace_irrel_pl : forall t tr1 tr1' tr2 e e' p1' p1 o' o,
-    well_formed t ->
+Lemma trace_irrel_pl : forall t tr1 tr1' tr2 e e' p1' p1,
+    well_formed_r t ->
     copland_compile t
-           {| st_ev := e;  st_trace := tr1; st_pl := p1;  st_store := o  |} =
-    (Some tt, {| st_ev := e'; st_trace := tr1'; st_pl := p1'; st_store := o' |}) ->
+           {| st_ev := e;  st_trace := tr1; st_pl := p1 (*;  st_store := o*)  |} =
+    (Some tt, {| st_ev := e'; st_trace := tr1'; st_pl := p1' (*; st_store := o'*) |}) ->
     
     st_pl
       (execSt (copland_compile t)
-           {| st_ev := e;  st_trace := tr2; st_pl := p1;  st_store := o  |}) = p1'.
+           {| st_ev := e;  st_trace := tr2; st_pl := p1 (*;  st_store := o*)  |}) = p1'.
 Proof.
   intros.
-  destruct (copland_compile t {| st_ev := e; st_trace := tr2; st_pl := p1; st_store := o |}) eqn:ff.
+  destruct (copland_compile t {| st_ev := e; st_trace := tr2; st_pl := p1(*; st_store := o*) |}) eqn:ff.
   simpl.
   vmsts.
   simpl.
@@ -572,18 +578,18 @@ Proof.
   tauto.
 Defined.
 
-Lemma trace_irrel_ev : forall t tr1 tr1' tr2 e e' p1' p1 o' o,
-    well_formed t ->
+Lemma trace_irrel_ev : forall t tr1 tr1' tr2 e e' p1' p1,
+    well_formed_r t ->
     copland_compile t
-           {| st_ev := e;  st_trace := tr1; st_pl := p1;  st_store := o  |} =
-    (Some tt, {| st_ev := e'; st_trace := tr1'; st_pl := p1'; st_store := o' |}) ->
+           {| st_ev := e;  st_trace := tr1; st_pl := p1 (*;  st_store := o*)  |} =
+    (Some tt, {| st_ev := e'; st_trace := tr1'; st_pl := p1' (*; st_store := o'*) |}) ->
     
     st_ev
       (execSt (copland_compile t)
-           {| st_ev := e;  st_trace := tr2; st_pl := p1;  st_store := o  |}) = e'.
+           {| st_ev := e;  st_trace := tr2; st_pl := p1 (*;  st_store := o*)  |}) = e'.
 Proof.
   intros.
-  destruct (copland_compile t {| st_ev := e; st_trace := tr2; st_pl := p1; st_store := o |}) eqn:ff.
+  destruct (copland_compile t {| st_ev := e; st_trace := tr2; st_pl := p1 (*; st_store := o*) |}) eqn:ff.
   simpl.
   vmsts.
   simpl.
