src/Main.v
@@ -27,11 +27,11 @@ Inductive traceS: St -> list Ev -> Prop :=
 | tconf: forall t tr p e,
     trace t p tr ->
     traceS (conf t p e) tr
-| trem: forall st tr j loc p,
+| trem: forall st tr j p,
     traceS st tr ->
-    traceS (rem j loc p st)
+    traceS (rem j p st)
            (tr ++
-               [(rpy (pred j) loc p (pl st))])
+               [(rpy (pred j) p (pl st))])
 | tls: forall st tr1 t tr2,
     traceS st tr1 ->
     trace t (pl st) tr2 ->
@@ -57,7 +57,7 @@ Fixpoint esizeS s:=
   match s with
   | stop _ _ => 0
   | conf t _ _ => esize t
-  | rem _ _ _ st => 1 + esizeS st
+  | rem _ _ st => 1 + esizeS st
   | ls st t => esizeS st + esize t
   (*| bsl _ st t _ _ => 1 + esizeS st + esize t
   | bsr _ _ st => 1 + esizeS st
