src/StVM.v
@@ -10,11 +10,11 @@ Require Import List.
 Import ListNotations.
 
 (* Specific VM monad state *)
-Definition ev_store := MapC nat EvidenceC.
+(*Definition ev_store := MapC nat EvidenceC. *)
 Record cvm_st : Type := mk_st
                          {st_ev:EvidenceC ;
                           st_trace:list Ev ;
-                          st_pl:Plc ;
-                          st_store:ev_store}.
+                          st_pl:Plc (*;
+                          st_store:ev_store*)}.
 
-Definition empty_vmst := mk_st mtc [] 0 [].
+Definition empty_vmst := mk_st mtc [] 0 (* [] *) .
